\documentclass[./main.tex]{subfiles}
\graphicspath{{\subfix{../Figures/}}}

\begin{document}

\appendix
\section*{Appendices}
\addcontentsline{toc}{section}{Appendices}
\renewcommand{\thesubsection}{\Alph{subsection}}

\subsection{Proofs}

\subsubsection{Solution for deterministic model}

\noindent \textbf{Budget constraints:}
\begin{align}
    \text{Young users: } && c_t^u &= e_t^u - s_t - (1+ \varphi_t^b+\varphi_t^v) q_t p_t - \hat{q}_t \hat{p}_t\\
    \text{Old users: } && c_{t+1}^u &=  s_t (1+r_t) + (1-h_{t+1})(1+\theta_{t+1}) q_t p_{t+1} + \hat{q}_t \hat{p}_{t+1} \\
    \text{Young validators: } && c_t^v &= e_t^v + \varphi_t^v q_t p_t - L_t p_t \\
    \text{Old validators: } && c_{t+1}^v &= (1+\delta_t) L_t p_{t+1} \\
    \text{Hackers: } && c_{t+1}^h &= h_{t+1} q_t p_{t+1}\\
\intertext{\textbf{Market clearing:}}
    \text{Risk-free assets: } && s_t &= 0\\
    \text{Tokens: } && q_t &= M_t - L_t\\
    \text{Fiat: } && \hat{q}_t &= m_t
\end{align}

\noindent \textbf{User's problem:}
\begin{equation}
    \begin{split}    
        \max_{s_t, q_t, \hat{q}_t}\quad & u\left(e_t^u - s_t - (1+ \varphi_t^b+\varphi_t^v) q_t p_t - \hat{q}_t \hat{p}_t\right)\\
        &+ \beta u\left(s_t (1+r_t) + (1-h_{t+1}) q_t p_{t+1} + \hat{q}_t \hat{p}_{t+1}\right)
    \end{split}
\end{equation}

FOCs:
\begin{align}
    \frac{\partial}{\partial s_t}: & -u'(c_t^u) + \beta(1+r_t)u'(c_{t+1}^u) = 0\\
    \frac{\partial}{\partial q_t}: & -(1+\varphi_t^b+\varphi_t^v) p_t u'(c_t^u) + \beta(1-h_{t+1})(1+\theta_{t+1})p_{t+1}u'(c_{t+1}^u) = 0 \\
    \frac{\partial}{\partial \hat{q}_t}: & -\hat{p}_t u'(c_t^u) + \beta \hat{p}_{t+1}u'(c_{t+1}^u) = 0
\end{align}

Euler's equations:
\begin{equation}
    \frac{u'(c_t^u)}{u'(c_{t+1}^u)} = \beta (1+r_t) 
    = \beta \frac{(1+\theta_{t+1})(1-h_{t+1})}{1+\varphi_t^b+\varphi_t^v} \frac{p_{t+1}}{p_t}
    = \beta \frac{\hat{p}_{t+1}}{\hat{p}_t}
\end{equation}

\noindent \textbf{Validator's problem:}
\begin{equation}
    \max_{L_t}\quad u(e_t^v + \varphi_t^v q_t p_t - L_t p_t) + \beta u((1+\delta_t) L_t p_{t+1})
\end{equation}

FOC:
\begin{equation}
    -p_t u'(c_t^v) + \beta p_{t+1} (1+\delta_t) u'(c_{t+1}^v) = 0
\end{equation}

Euler's equation:
\begin{equation}
    \frac{u'(c_t^v)}{u'(c_{t+1}^v)} = \beta (1+\delta_t) \frac{p_{t+1}}{p_t}
\end{equation}

\paragraph{Token market equilibrium with log utility}

\begin{equation}
    u(c_t) = \ln c_t \Rightarrow \frac{u'(c_t)}{u'(c_{t+1})} = \frac{c_{t+1}}{c_t}
\end{equation}

\noindent \textbf{Users' equilibrium token holding:}
\begin{align}
    \intertext{By users' BC\textcircled{2}:}
    \hat{q}_t &= \frac{1}{\hat{p}_{t+1}}\left[c_{t+1}^u -  s_t (1+r_t) - (1-h_{t+1})(1+\theta_{t+1}) q_t p_{t+1} \right]\\
    \intertext{Substitute into users' BC\textcircled{1}, eliminate $s_t$ by market clearing:}
    c_t^u &= e_t^u - (1+ \varphi_t^b+\varphi_t^v) q_t p_t - \frac{\hat{p}_t}{\hat{p}_{t+1}}\left[c_{t+1}^u - (1-h_{t+1})(1+\theta_{t+1}) q_t p_{t+1} \right]\\
    \intertext{By users' FOC\textcircled{3}:} 
    \frac{c_{t+1}^u}{c_t^u}&=\beta\frac{\hat{p}_{t+1}}{\hat{p}_t} \Rightarrow \frac{\hat{p}_t}{\hat{p}_{t+1}}c_{t+1}^u = \beta c_t^u \\
    \intertext{Eliminate $c_{t+1}^u$ :}
    c_t^u(1+\beta) &= e_t^u - (1+ \varphi_t^b+\varphi_t^v) q_t p_t + \frac{\hat{p}_t}{\hat{p}_{t+1}}(1-h_{t+1})(1+\theta_{t+1}) q_t p_{t+1}\\
    \intertext{Substitute users' BC\textcircled{1} and $s_t=0,\hat{q}_t=m_t$ on LHS:}
    &(1+\beta)\left[ e_t^u - (1+ \varphi_t^b+\varphi_t^v) q_t p_t - m_t \hat{p}_t \right] \nonumber \\ 
    &= e_t^u - (1+ \varphi_t^b+\varphi_t^v) q_t p_t + \frac{\hat{p}_t}{\hat{p}_{t+1}}(1-h_{t+1})(1+\theta_{t+1}) q_t p_{t+1}\\
    \intertext{Merge terms:}
    \beta e_t^u - (1+\beta)m_t\hat{p}_t &= q_t p_t \left[\beta(1+ \varphi_t^b+\varphi_t^v) + \frac{\hat{p}_t}{\hat{p}_{t+1}}(1-h_{t+1})(1+\theta_{t+1}) \frac{p_{t+1}}{p_t}\right]
\end{align}
Hence the inverse demand curve is
\begin{equation}
    q_t = \left[ \beta \frac{e_t^u}{p_t} - (1+\beta)m_t \frac{\hat{p}_t}{p_t} \right]
    \left[\beta(1+ \varphi_t^b+\varphi_t^v) + \frac{(1-h_{t+1})(1+\theta_{t+1})}{1+r_t} \frac{p_{t+1}}{p_t}\right]^{-1}
\end{equation}


\noindent \textbf{Validators' equilibrium staking:}
\begin{align}
    \frac{c_{t+1}^v}{c_t^v} = \frac{(1+\delta_t) L_t p_{t+1}}{e_t^v + \varphi_t^v q_t p_t - L_t p_t} &= \beta (1+\delta_t) \frac{p_{t+1}}{p_t}\\
    L_t &= \beta \left(\frac{e_t^v}{p_t} + \varphi_t^v q_t - L_t\right)\\
    L_t &= \frac{\beta}{1+\beta} \left(\frac{e_t^v}{p_t} + \varphi_t^v q_t\right)\\
    \intertext{By market clearing $q_t+L_t=M_t$:}
    q_t+\frac{\beta}{1+\beta} \left(\frac{e_t^v}{p_t} + \varphi_t^v q_t\right) &= M_t\\
    q_t\left(1+\frac{\beta}{1+\beta}\varphi_t^v\right) &= M_t - \frac{\beta}{1+\beta}\frac{e_t^v}{p_t}
\end{align}
Hence the inverse supply curve is
\begin{equation}
    q_t = \left(1+\frac{\beta}{1+\beta}\varphi_t^v\right)^{-1} \left(M_t - \frac{\beta}{1+\beta}\frac{e_t^v}{p_t}\right)
\end{equation}

\noindent \textbf{Token market equilibrium:}\\
Let $p_t^*$ be the equilibrium price of crypto tokens. $p_t^*$ must satisfy:
\begin{align}
    & \left[ \beta \frac{e_t^u}{p_t^*} - (1+\beta)m_t \frac{\hat{p}_t}{p_t^*} \right]
    \left[\beta(1+ \varphi_t^b+\varphi_t^v) + \frac{(1-h_{t+1})(1+\theta_{t+1})}{1+r_t} \frac{p_{t+1}}{p_t^*}\right]^{-1} \nonumber \\
    &= \left(1+\frac{\beta}{1+\beta}\varphi_t^v\right)^{-1} \left(M_t - \frac{\beta}{1+\beta}\frac{e_t^v}{p_t^*}\right)
    \intertext{which can be alternatively written as a quardatic function of $\frac{1}{p_t^*}$:}
    A_t \frac{1}{p_t^*} &= (M_t + B_t\frac{1}{p_t^*}) (C_t + D_t\frac{1}{p_t^*}) \\
    \intertext{where}
    A_t &:= \left[ \beta e_t^u - (1+\beta)m_t \hat{p}_t \right] \left(1+\frac{\beta}{1+\beta}\varphi_t^v\right);\\
    B_t &:= - \frac{\beta}{1+\beta} e_t^v;\\
    C_t &:= \beta(1+ \varphi_t^b+\varphi_t^v);\\
    D_t &:= \frac{(1-h_{t+1})(1+\theta_{t+1})}{1+r_t} p_{t+1}
    \intertext{Therefore the closed-form solution for equilibrium token price is given by}
    p_t^* &= \frac{2B_tD_t}{A_t-M_t D_t-B_tC_t - \sqrt{(M_t D_t+B_t C_t-A_t)^2-4M_t B_tC_tD_t}}\\
    \intertext{under the following technical conditions:}
    4M_t B_tC_tD_t &\leq (M_t D_t+B_t C_t-A_t)^2\\
    A_t-M_t D_t-B_tC_t &\neq \sqrt{(M_t D_t+B_t C_t-A_t)^2-4M_t B_tC_tD_t}
\end{align}

\end{document}